CMessage
add support for HTTP operations in the spec

ironfleet/src/Dafny/Distributed/Services/WS/WS.s.dfy
@@ -4,18 +4,21 @@ module WS__WS_s {
 
 import opened Native__Io_s
 
-datatype Request = Request(fileName:seq<char>)
-datatype Response = ResponseValid(r:seq<byte>) | Response404()
+type HTTPRequest = seq<char>
+datatype HTTPResponse = ResponseValid(r:seq<byte>) | Response404()
 
 predicate SpecInit()
 {
     true
 }
 
-predicate Get(fs:FileSystemState, req:Request, res:Response)
+predicate Get(fs:FileSystemState, req:HTTPRequest, res:HTTPResponse)
     requires fs != null;
 {
        fs != null
-    && (res == if fs.file_exists(req.fileName) then ResponseValid(fs.contents(req.fileName)) else Response404())
+    && (exists op,filePath,ver :: (req == op + " " + filePath + " " + ver) 
+                               && op == "GET" && |filePath| > 1 
+                               && ver == "HTTP/1.0" 
+                               && (res == if fs.file_exists(filePath) then ResponseValid(fs.contents(filePath[1..])) else Response404()))
 }
 }
