ironfleet/src/Dafny/Distributed/Impl/WS/CMessage.i.dfy
@@ -1,0 +1,102 @@
+include "../../Protocol/WS/Message.i.dfy"
+include "../Common/NodeIdentity.i.dfy"
+include "../../Protocol/WS/Network.i.dfy"
+include "Parameters.i.dfy"
+include "../../Common/Logic/Option.i.dfy"
+
+module WS__CMessage_i {
+import opened WS__Message_i
+import opened Common__NodeIdentity_i
+import opened WS__Network_i
+import opened Impl_Parameters_i
+import opened Logic__Option_i
+
+datatype CMessage =
+      CGetRequest(req:Request)
+    | CGetResponse(response:Response)
+    
+
+datatype CPacket = CPacket(dst:EndPoint, src:EndPoint, msg:CMessage)
+
+predicate CMessageIsAbstractable(cmsg:CMessage)
+{
+    true
+}
+
+function AbstractifyCMessageToMessage(cmsg:CMessage) : Message
+    requires CMessageIsAbstractable(cmsg);
+{
+    match cmsg
+        case CGetRequest(req) => GetRequest(req)
+        case CGetResponse(resp) => GetResponse(resp)
+}
+
+predicate CMessageSeqIsAbstractable(cs:seq<CMessage>)
+{
+    forall m :: m in cs ==> CMessageIsAbstractable(m)
+}
+
+function AbstractifySeqOfCMessageToSeqOfMessage(cs:seq<CMessage>) : seq<Message>
+    requires CMessageSeqIsAbstractable(cs);                                          
+{
+    MapSeqToSeq(cs, AbstractifyCMessageToMessage)
+}
+
+//////////////////////////////////////////////////////////////////////////////
+
+predicate CPacketIsAbstractable(cpacket:CPacket)
+{
+       EndPointIsAbstractable(cpacket.dst)
+    && EndPointIsAbstractable(cpacket.src)
+    && CMessageIsAbstractable(cpacket.msg)
+}
+
+function AbstractifyCPacketToShtPacket(cpacket:CPacket) : Packet
+    requires CPacketIsAbstractable(cpacket);
+{
+    Packet(AbstractifyEndPointToNodeIdentity(cpacket.dst),
+           AbstractifyEndPointToNodeIdentity(cpacket.src),
+           AbstractifyCMessageToMessage(cpacket.msg))
+}
+
+predicate CPacketsIsAbstractable(cps:set<CPacket>)
+{
+    forall p :: p in cps ==> CPacketIsAbstractable(p)
+}
+
+function {:opaque} AbstractifyCPacketsToPackets(cps:set<CPacket>) : set<Packet>
+    requires CPacketsIsAbstractable(cps);
+    ensures forall p :: p in cps ==> AbstractifyCPacketToShtPacket(p) in AbstractifyCPacketsToPackets(cps);
+{
+    set p | p in cps :: AbstractifyCPacketToShtPacket(p)
+}
+
+predicate CPacketSeqIsAbstractable(cps:seq<CPacket>)
+{
+    forall p :: p in cps ==> CPacketIsAbstractable(p)
+}
+
+function {:opaque} AbstractifySeqOfCPacketsToSetOfShtPackets(cps:seq<CPacket>) : set<Packet>
+    requires CPacketSeqIsAbstractable(cps);
+    ensures forall p :: p in cps ==> AbstractifyCPacketToShtPacket(p) in AbstractifySeqOfCPacketsToSetOfShtPackets(cps);
+{
+    set p | p in cps :: AbstractifyCPacketToShtPacket(p)
+}
+
+predicate OptionCPacketIsAbstractable(cp:Option<CPacket>)
+{
+    match cp {
+        case Some(p) => CPacketIsAbstractable(p)
+        case None => true
+    }
+}
+
+function AbstractifyOptionCPacketToOptionShtPacket(cp:Option<CPacket>) : Option<Packet>
+    requires OptionCPacketIsAbstractable(cp);
+{
+    match cp {
+        case Some(p) => Some(AbstractifyCPacketToShtPacket(p))
+        case None => None()
+    }
+}
+}
