ironfleet/src/Dafny/Distributed/Protocol/SHT/Parameters.i.dfy
@@ -1,4 +1,4 @@
-module Protocol_Parameters_i {
+module WSProtocol_Parameters_i {
 
 datatype Parameters = Parameters(max_seqno:nat, max_delegations:nat)
 
